Reframing all results for journal version (with one hole)

Maps.v
@@ -148,6 +148,9 @@ Fixpoint Beval (V:Valuation) (e:Bexpr) : bool :=
   | BLeq a1 a2 => (Aeval V a1) <=? (Aeval V a2)
   end.
 
+Notation "V |= b" := (Beval V b = true) (at level 90).
+Notation "V |/= b" := (Beval V b = false) (at level 90).
+
 (** We can update a valuation with a substitution by composition
       and prove some useful properties *)
 
@@ -182,3 +185,144 @@ Qed.
 Lemma comp_id : forall V,
     Comp V id_sub = V.
 Proof. intros. extensionality x. reflexivity. Qed.
+
+Definition denot_sub (phi: sub): Valuation -> Valuation := fun V => Comp V phi.
+Notation "[| s |]" := (denot_sub s).
+
+Lemma denot_id_sub: denot_sub id_sub = fun V => V.
+Proof. unfold denot_sub. extensionality V. rewrite comp_id. reflexivity. Qed.
+
+Definition compose_subs (s s': sub): sub := fun x => Aapply s (s' x).
+
+Lemma compose_subs_id: forall s, compose_subs id_sub s = s.
+Proof.
+  intros.
+  unfold compose_subs.
+  extensionality x.
+  now rewrite Aapply_id.
+Qed.
+
+Lemma compose_subs_id': forall s, compose_subs s id_sub = s.
+Proof.
+  intros.
+  unfold compose_subs.
+  extensionality x.
+  easy.
+Qed.
+
+Lemma compose_subs_assoc: forall σ1 σ2 σ3,
+    compose_subs σ1 (compose_subs σ2 σ3) = compose_subs (compose_subs σ1 σ2) σ3.
+Proof.
+  intros.
+  extensionality y.
+  unfold compose_subs.
+  induction (σ3 y); cbn; auto.
+  now rewrite IHa1, IHa2.
+Qed.
+
+Lemma compose_comp: forall V s s',
+    Comp V (compose_subs s s') = (fun x => Comp (Comp V s) s' x).
+Proof.
+  intros.
+  extensionality x.
+  unfold Comp, compose_subs.
+  induction (s' x); simpl; auto.
+Qed.
+
+Lemma compose_sub_spec: forall s1 s2,
+    [| compose_subs s1 s2 |] = fun V => [| s2 |] ([| s1 |] V).
+Proof.
+  intros.
+  extensionality V.
+  unfold denot_sub.
+  now rewrite compose_comp.
+Qed.
+
+Lemma asgn_compose: forall σ x e,
+    (update σ x (Aapply σ e)) = compose_subs σ (x !-> e ; id_sub).
+Proof.
+  intros.
+  extensionality y.
+  unfold compose_subs, update.
+  now destruct (eqb x y).
+Qed.
+
+Lemma asgn_compose': forall σ σ' x e,
+    (x !-> Aapply (compose_subs σ σ') e; compose_subs σ σ') = compose_subs σ (x !-> Aapply σ' e; σ').
+Proof.
+  intros.
+  extensionality y.
+  unfold compose_subs, update.
+  destruct (eqb x y); auto.
+  induction e; cbn; auto.
+  now rewrite IHe1, IHe2.
+Qed.
+
+Lemma Aapply_compose: forall σ σ' e,
+    Aapply σ (Aapply σ' e) = Aapply (compose_subs σ σ') e.
+Proof.
+  intros.
+  induction e; auto; cbn.
+  now rewrite IHe1, IHe2.
+Qed.
+
+Lemma Bapply_compose: forall σ σ' b,
+    Bapply σ (Bapply σ' b) = Bapply (compose_subs σ σ') b.
+Proof.
+  intros.
+  induction b; cbn; auto.
+  - now rewrite IHb.
+  - now rewrite IHb1, IHb2.
+  - now rewrite 2 Aapply_compose.
+Qed.
+
+From Coq Require Import Ensembles.
+Definition denot__B (b: Bexpr): Ensemble Valuation := fun V => Beval V b = true.
+Notation "{| b |}" := (denot__B b).
+Open Scope com_scope.
+
+(* Characterizing denot__B *)
+Lemma denotB_true: forall V b, In _ (denot__B b) V <-> Beval V b = true.
+Proof. split; intros; apply H. Qed.
+
+Lemma denotB_false: forall V b, In _ (Complement _ (denot__B b)) V <-> Beval V b = false.
+Proof.
+    split; intros.
+    - apply (not_true_is_false _ H).
+    - unfold Complement, In, denot__B. intro. rewrite H in H0. discriminate.
+Qed.
+
+Lemma denotB_top: denot__B (BTrue) = Full_set _.
+Proof.
+  apply Extensionality_Ensembles. split; intros V _.
+  - apply Full_intro.
+  - unfold denot__B, In. reflexivity.
+Qed.
+
+Lemma denotB_bot: denot__B BFalse = Empty_set _.
+Proof. apply Extensionality_Ensembles. split; intros V H; inversion H. Qed.
+
+Lemma denotB_neg: forall b, denot__B <{~ b}> = Complement _ (denot__B b).
+Proof.
+  intros. apply Extensionality_Ensembles. split; intros V H.
+  - intro contra. inversion H. inversion contra.
+    rewrite negb_true_iff in H1. rewrite H1 in H2. discriminate.
+  - unfold denot__B, Ensembles.In. simpl. rewrite negb_true_iff.
+    apply not_true_is_false in H. apply H.
+Qed.
+
+Lemma denotB_and: forall b1 b2,
+    denot__B <{b1 && b2}> = Intersection _ (denot__B b1) (denot__B b2).
+Proof.
+  intros. apply Extensionality_Ensembles. split; intros V H.
+  - inversion H. apply andb_true_iff in H1. destruct H1.
+    split; assumption.
+  - destruct H.
+    unfold denot__B, Ensembles.In. simpl. rewrite andb_true_iff.
+    split; assumption.
+Qed.
+
+Create HintDb denotB.
+
+#[export] Hint Rewrite denotB_true denotB_false denotB_top denotB_bot denotB_neg denotB_and
+  : denotB.
