Syntax.v
@@ -1,47 +1,102 @@
 From Coq Require Import Strings.String.
 From BigStepSymbEx Require Import Expr.
 
-Module While.
-  Inductive Stmt : Type :=
-  | SSkip
-  | SAsgn (x:string) (e:Aexpr)
-  | SSeq (s1 s2:Stmt)
-  | SIf (b:Bexpr) (s1 s2:Stmt)
-  | SWhile (b:Bexpr) (s:Stmt).
+Module Trace.
+  Inductive Trc : Type :=
+  | TSkip
+  | TAsgn (x:string) (e:Aexpr)
+  | TAsrt (b:Bexpr)
+  | TSeq (t1 t2: Trc).
+End Trace.
 
-  Notation "'skip'" := SSkip (in custom com at level 80) : com_scope.
+Module TraceNotations.
+  Import Trace.
+
+  Notation "'skip'" := TSkip (in custom com at level 80) : com_scope.
   Notation "x := y"  :=
-          (SAsgn x y)
-              (in custom com at level 0, x constr at level 0,
-              y at level 85, no associativity) : com_scope.
+    (TAsgn x y)
+      (in custom com at level 0, x constr at level 0,
+          y at level 85, no associativity) : com_scope.
+  Notation "b ?" :=
+    (TAsrt b)
+      (in custom com at level 90, right associativity) : com_scope.
   Notation "x ; y" :=
-          (SSeq x y)
-            (in custom com at level 90, right associativity) : com_scope.
-  Notation "'if' x '{' y '}' '{' z '}'" :=
-          (SIf x y z)
-            (in custom com at level 89, x at level 99,
-              y at level 99, z at level 99) : com_scope.
-  Notation "'while' x '{' y '}'" :=
-          (SWhile x y)
-            (in custom com at level 89, x at level 99,
-              y at level 99) : com_scope.
+    (TSeq x y)
+      (in custom com at level 90, right associativity) : com_scope.
+End TraceNotations.
 
+Module NonDet.
+  Inductive Prg : Type :=
+  | PSkip
+  | PAsgn (x:string) (e:Aexpr)
+  | PAsrt (b:Bexpr)
+  | PSeq (p1 p2: Prg)
+  | PChoice (p1 p2: Prg)
+  | PStar (p: Prg)
+  .
+
+  Axiom Prg_assoc: forall p q r, PSeq p (PSeq q r) = PSeq (PSeq p q) r.
+End NonDet.
+
+Module NonDetNotations.
+  Import NonDet.
+
+  Notation "'skip'" := PSkip (in custom com at level 80) : com_scope.
+  Notation "x := y"  :=
+    (PAsgn x y)
+      (in custom com at level 0, x constr at level 0,
+          y at level 85, no associativity) : com_scope.
+  Notation "b ?" :=
+    (PAsrt b)
+      (in custom com at level 90, right associativity) : com_scope.
+  Notation "x ; y" :=
+    (PSeq x y)
+      (in custom com at level 90, right associativity) : com_scope.
+  Notation "x (+) y" :=
+    (PChoice x y)
+      (in custom com at level 90, right associativity) : com_scope.
+  Notation "x *" :=
+    (PStar x)
+      (in custom com at level 90, right associativity) : com_scope.
   Open Scope com_scope.
+End NonDetNotations.
 
-  Lemma seq_discriminate1: forall p q, p <> <{p ; q}>.
-  Proof. intros p q contra. induction p;
-           try discriminate.
-         inversion contra; subst. apply IHp1; assumption.
-  Qed.
+Section While.
+Import NonDet NonDetNotations.
 
-  Lemma seq_discriminate2: forall p q, q <> <{p ; q}>.
-  Proof. intros p q contra. induction q;
-           try discriminate.
-         inversion contra; subst. apply IHq2; assumption.
-  Qed.
+Inductive Stmt: Type :=
+| Skip
+| Asgn (x:string) (e:Aexpr)
+| Seq (s1 s2: Stmt)
+| If (b:Bexpr) (s1 s2: Stmt)
+| While (b:Bexpr) (s: Stmt).
 
-  Definition X: string := "x".
-  Definition Y: string := "y".
-  Definition Z: string := "z".
-
+Fixpoint encode (s:Stmt): Prg :=
+  match s with
+  | Skip => PSkip
+  | Asgn x e => PAsgn x e
+  | Seq s1 s2 => PSeq (encode s1) (encode s2)
+  | If b s1 s2 => PChoice (PSeq <{b?}> (encode s1)) (PSeq <{~b?}> (encode s2))
+  | While b s => PSeq (PStar (PSeq <{b?}> (encode s))) <{~b?}>
+  end.
 End While.
+
+Module WhileNotations.
+
+  Notation "'skip'" := Skip (in custom com at level 80) : com_scope.
+  Notation "x := y"  :=
+    (Asgn x y)
+      (in custom com at level 0, x constr at level 0,
+          y at level 85, no associativity) : com_scope.
+  Notation "x ; y" :=
+    (Seq x y)
+      (in custom com at level 90, right associativity) : com_scope.
+  Notation "'if' x '{' y '}' '{' z '}'" :=
+    (If x y z)
+      (in custom com at level 89, x at level 99,
+          y at level 99, z at level 99) : com_scope.
+  Notation "'while' x '{' y '}'" :=
+    (While x y)
+      (in custom com at level 89, x at level 99,
+          y at level 99) : com_scope.
+End WhileNotations.
