Operational.v
@@ -1,0 +1,494 @@
+From Coq Require Import
+  Program.Equality
+  Relations
+  Classes.RelationClasses
+  Logic.FunctionalExtensionality
+  Ensembles.
+
+From BigStepSymbEx Require Import
+  Utils
+  Expr
+  Syntax
+  Maps
+  Programs
+  Traces
+.
+Import Trace.
+Import NonDet NonDetNotations.
+
+Open Scope com_scope.
+
+Definition SConfig : Type := Prg * sub * Bexpr.
+
+Reserved Notation " c '->s' c' " (at level 40).
+
+(* Figure 3 *)
+Inductive Sstep : relation SConfig :=
+| Asgn_step : forall x e sig phi,
+    (<{ x := e }>, sig , phi) ->s (PSkip, (update sig x (Aapply sig e)), phi)
+| Asrt_step : forall b sig phi,
+    (<{ b? }>, sig, phi) ->s (PSkip, sig, BAnd phi (Bapply sig b))
+| Skip_step : forall p sig phi,
+    (<{skip ; p}>, sig, phi) ->s (p, sig, phi)
+| Seq_step : forall p p' q sig sig' phi phi',
+    (p, sig, phi) ->s (p', sig', phi') ->
+    (<{p ; q}>, sig, phi) ->s (<{p' ; q}>, sig', phi')
+| Ndet_step_l : forall p q sig phi,
+    (<{p (+) q}>, sig, phi) ->s (p, sig, phi)
+| Ndet_step_r : forall p q sig phi,
+    (<{p (+) q}>, sig, phi) ->s (q, sig, phi)
+| Loop_step_halt : forall p sig phi,
+    (<{p*}>, sig, phi) ->s (PSkip, sig, phi)
+| Loop_step_unfold: forall p sig phi,
+    (<{p*}>, sig, phi) ->s (<{p ; p*}>, sig, phi)
+  where " c '->s' c' " := (Sstep c c').
+
+Lemma Asgn': forall p q σ σ' φ φ' x e,
+    p = <{x := e}> ->
+    q = PSkip ->
+    σ' = (update σ x (Aapply σ e)) ->
+    φ' = φ ->
+    (p, σ, φ) ->s (q, σ', φ').
+Proof.
+  intros.
+  subst.
+  apply Asgn_step.
+Qed.
+
+Lemma Asrt': forall p q σ σ' φ φ' b,
+    p = <{b?}> ->
+    q = PSkip ->
+    σ' = σ ->
+    φ' = BAnd φ (Bapply σ b) ->
+    (p, σ, φ) ->s (q, σ', φ').
+Proof.
+  intros.
+  subst.
+  apply Asrt_step.
+Qed.
+
+Definition multi_Sstep := clos_refl_trans_n1 _ Sstep.
+Notation " c '->*' c' " := (multi_Sstep c c') (at level 40).
+
+(* Lemma 10 *)
+Lemma if_T: forall b p q sig phi,
+    (encode (If b p q), sig, phi) ->* (encode p, sig, BAnd phi (Bapply sig b)).
+Proof.
+  cbn;intros.
+  apply clos_rt1n_rtn1.
+  econstructor.
+  { apply Ndet_step_l. }
+  econstructor.
+  { do 2 constructor. }
+  econstructor.
+  { do 2 constructor. }
+  constructor.
+Qed.
+
+Lemma if_F: forall b p q sig phi,
+    (encode (If b p q), sig, phi) ->* (encode q, sig, BAnd phi (Bapply sig <{~b}>)).
+Proof.
+  cbn;intros.
+  apply clos_rt1n_rtn1.
+  econstructor.
+  { apply Ndet_step_r. }
+  econstructor.
+  { do 2 constructor. }
+  econstructor.
+  { do 2 constructor. }
+  constructor.
+Qed.
+
+Lemma while_T: forall b p sig phi,
+    (encode (While b p), sig, phi) ->* (encode (Seq p (While b p)), sig, BAnd phi (Bapply sig b)).
+Proof.
+  cbn;intros.
+  apply clos_rt1n_rtn1.
+  econstructor.
+  { econstructor; apply Loop_step_unfold. }
+  econstructor.
+  { do 3 econstructor.
+    apply Asrt_step.
+  }
+  econstructor.
+  { do 3 constructor. }
+  rewrite Prg_assoc. (*<- note this dependence on syntactic associativity of Seq *)
+  constructor.
+Qed.
+
+Lemma while_F: forall b p sig phi,
+    (encode (While b p), sig, phi) ->* (encode Skip, sig, BAnd phi (Bapply sig <{~b}>)).
+Proof.
+  cbn;intros.
+  apply clos_rt1n_rtn1.
+  econstructor.
+  { econstructor; apply Loop_step_halt. }
+  econstructor.
+  { constructor. }
+  econstructor.
+  { constructor. }
+  now constructor.
+Qed.
+
+Definition In': Ensemble Branch -> Branch -> Prop :=
+  fun F '(σ, φ) => exists φ', In _ F (σ, φ') /\ {| φ |} = {| φ' |}.
+
+Definition multi_Sstep': relation SConfig :=
+  fun '(p, σ, φ) '(q, σ', φ') => exists φ'', (p, σ, φ) ->* (q, σ', φ'') /\ {| φ'' |} = {| φ' |}.
+Notation " c '=>*' c' " := (multi_Sstep' c c') (at level 40).
+
+(*NOTE: Erik claims iff, but I don't think the condition on φ is strong enough *)
+Lemma canonical_SE_step: forall p q σ σ' φ φ',
+    (p, σ, φ) ->s (q, σ', φ') -> exists σc φc,
+        (p, id_sub, BTrue) ->s (q, σc, φc)
+      /\ (σ' = compose_subs σ σc)
+      /\ ({| φ' |} = {| BAnd φ (Bapply σ φc) |}).
+Proof.
+  intros.
+  dependent induction H.
+  + eexists. eexists.
+    splits.
+    * constructor.
+    * rewrite Aapply_id.
+      now rewrite asgn_compose.
+    * cbn.
+      now rewrite denotB_and, denotB_top, intersect_comm, intersect_full.
+  + eexists. exists (BAnd BTrue (Bapply id_sub b)).
+    splits.
+    * constructor.
+    * now rewrite compose_subs_id'.
+    * cbn.
+      now rewrite Bapply_id, 3 denotB_and, denotB_top, intersect_full.
+  + eexists. eexists.
+    splits.
+    * constructor.
+    * now rewrite compose_subs_id'.
+    * cbn.
+      now rewrite denotB_and, denotB_top, intersect_comm, intersect_full.
+  + pose proof IHSstep _ _ _ _ _ _ JMeq_refl JMeq_refl as (σc & φc & ? & ? & ?).
+    eexists. eexists.
+    splits.
+    * constructor; eauto.
+    * assumption.
+    * assumption.
+  + eexists. eexists.
+    splits.
+    * apply Ndet_step_l.
+    * now rewrite compose_subs_id'.
+    * cbn.
+      now rewrite denotB_and, denotB_top, intersect_comm, intersect_full.
+
+  + eexists. eexists.
+    splits.
+    * apply Ndet_step_r.
+    * now rewrite compose_subs_id'.
+    * cbn.
+      now rewrite denotB_and, denotB_top, intersect_comm, intersect_full.
+
+  + eexists. eexists.
+    splits.
+    * apply Loop_step_halt.
+    * now rewrite compose_subs_id'.
+    * cbn.
+      now rewrite denotB_and, denotB_top, intersect_comm, intersect_full.
+
+  + eexists. eexists.
+    splits.
+    * apply Loop_step_unfold.
+    * now rewrite compose_subs_id'.
+    * cbn.
+      now rewrite denotB_and, denotB_top, intersect_comm, intersect_full.
+Qed.
+
+Lemma canonical_soundness_step: forall p q σ φ σ' φ',
+    (p, id_sub, BTrue) ->s (q, σ, φ) ->
+    In _ (denot__S q) (σ', φ') ->
+    In' (denot__S p) (compose_subs σ σ', BAnd φ (Bapply σ φ')).
+Proof.
+  induction p; intros; inv H.
+  - destruct H0 as (?t & ? & -> & ->).
+    inv H0; cbn in *.
+    exists BTrue.
+    splits.
+    exists (TAsgn x e).
+    splits; cbn.
+    now rewrite asgn_compose, compose_subs_id, compose_subs_id'.
+
+  - destruct H0 as (?t & ? & -> & ->).
+    inv H0; cbn in *.
+    exists <{ b }>.
+    split.
+    + exists (TAsrt b).
+      splits.
+    + now rewrite 2 denotB_and, Bapply_id, denotB_top, intersect_full, intersect_comm, intersect_full.
+
+  - exists φ'.
+    split.
+    + rewrite compose_subs_id.
+      destruct H0 as (?t & ? & -> & ->).
+      exists t.
+      splits.
+      exists TSkip, t.
+      splits; auto.
+      now rewrite trace_app_unit_l.
+    + now rewrite Bapply_id, denotB_and, denotB_top, intersect_full.
+
+  - destruct H0 as (?t & ? & -> & ->).
+    destruct H0 as (?u & ?v & ? & ? & ->).
+    assert (In _ (denot__S p') (Sub u, PC u)). {
+      eexists; splits; eauto.
+    }
+    epose proof IHp1 _ _ _ _ _ H2 H3 as (?φ & ? & ?).
+    destruct H4 as (?t & ? & ? & ->).
+    exists (PC (trace_app t v)).
+    split.
+    + exists (trace_app t v).
+      splits.
+      * exists t,v.
+        splits; auto.
+      * now rewrite 2 sub_trace_app, <- H6, compose_subs_assoc.
+    + rewrite concat_pc.
+      rewrite 2 denotB_and.
+      rewrite <- H5, <- H6.
+      rewrite denotB_and.
+      rewrite 3 inverse_denotB.
+      rewrite concat_pc.
+      rewrite denotB_and.
+      rewrite inverse_denotB.
+      rewrite compose_sub_spec.
+      rewrite <- intersect_assoc.
+      rewrite inverse_intersection.
+      now rewrite inverse_inverse.
+  (* ^eww, but it works *)
+
+  - exists φ'.
+    split.
+    + rewrite compose_subs_id.
+      destruct H0 as (?t & ? & -> & ->).
+      exists t.
+      splits.
+      left; auto.
+    + now rewrite Bapply_id, denotB_and, denotB_top, intersect_full.
+
+  - exists φ'.
+    split.
+    + rewrite compose_subs_id.
+      destruct H0 as (?t & ? & -> & ->).
+      exists t.
+      splits.
+      right; auto.
+    + now rewrite Bapply_id, denotB_and, denotB_top, intersect_full.
+
+  - destruct H0 as (?t & ? & -> & ->).
+    inv H0.
+    rewrite compose_subs_id.
+    exists BTrue.
+    splits.
+    eexists.
+    splits; auto.
+    exists 0; auto.
+
+
+  - exists φ'.
+    split.
+    + rewrite compose_subs_id.
+      destruct H0 as (?t & ? & -> & ->).
+      rewrite denotS_spec_unfold.
+      right.
+      exists t.
+      splits; auto.
+    + now rewrite Bapply_id, denotB_and, denotB_top, intersect_full.
+Qed.
+
+(* Corollary 1 *)
+Corollary canonical_soundness: forall p q σ σ' φ φ',
+    (p, id_sub, BTrue) ->* (q, σ, φ) ->
+    In _ (denot__S q) (σ', φ') ->
+    In' (denot__S p) (compose_subs σ σ', BAnd φ (Bapply σ φ')).
+Proof.
+  intros p q σ σ' φ φ' ? ?.
+  generalize dependent σ'.
+  generalize dependent φ'.
+  dependent induction H; intros.
+  - destruct H0 as (?t & ? & -> & ->).
+    exists (PC t).
+    splits.
+    exists t.
+    splits; auto.
+    + now rewrite compose_subs_id.
+    + now rewrite Bapply_id, denotB_and, denotB_top, intersect_full.
+  - destruct y as ((? & ?) & ?).
+    apply canonical_SE_step in H.
+    destruct H as (?σ & ?φ & ? & -> & ?).
+    epose proof canonical_soundness_step _ _ _ _ _ _ H H1 as (?φ & ? & ?).
+    epose proof IHclos_refl_trans_n1 _ _ _ _ JMeq_refl JMeq_refl _ _ H3 as (?φ & ? & ?).
+    exists φ2.
+    split.
+    + now rewrite <- compose_subs_assoc.
+    + rewrite <- H6.
+      rewrite 2 denotB_and.
+      rewrite 2 inverse_denotB.
+      rewrite <- H4, H2.
+      rewrite 2 denotB_and.
+      rewrite 2 inverse_denotB.
+      rewrite inverse_intersection.
+      rewrite inverse_inverse.
+      rewrite compose_sub_spec.
+      now rewrite <- intersect_assoc.
+Qed.
+
+(* Theorem 4 *)
+Theorem soundness: forall p σ φ,
+    (p, id_sub, BTrue) ->* (PSkip, σ, φ) ->
+    In' (denot__S p) (σ, φ).
+Proof.
+  intros.
+  assert (In _ (denot__S <{ skip }>) (id_sub, BTrue)) by (exists TSkip; split; easy).
+  epose proof canonical_soundness _ _ _ _ _ _ H H0 as (?φ & ? & ?).
+  eexists φ0.
+  split; eauto.
+  rewrite <- H2; cbn.
+  now rewrite denotB_and, denotB_top, intersect_comm, intersect_full.
+Qed.
+
+Lemma trace_to_denotS: forall p t,
+    In _ (traces_of p) t ->
+    In _ (denot__S p) (Sub t, PC t).
+Proof.
+  intros.
+  exists t; now splits.
+Qed.
+
+Lemma seq_star: forall p1 p2 q σ1 σ2 φ1 φ2,
+    (p1, σ1, φ1) ->* (p2, σ2, φ2) ->
+    (<{p1 ; q}>, σ1, φ1) ->* (<{p2 ; q}>, σ2, φ2).
+Proof.
+  intros.
+  dependent induction H.
+  - constructor.
+  - destruct y as ((? & ?) &?).
+    econstructor.
+    + now apply Seq_step; eauto.
+    + now apply IHclos_refl_trans_n1.
+Qed.
+
+Lemma seq_canonical: forall p1 p2 σ1 σ2 φ1 φ2,
+    (p1, id_sub, BTrue) ->* (PSkip, σ1, φ1) ->
+    (p2, id_sub, BTrue) ->* (PSkip, σ2, φ2) ->
+    (<{ p1; p2 }>, id_sub, BTrue) =>*
+      (<{ skip }>, compose_subs σ1 σ2, BAnd φ1 (Bapply σ1 φ2)).
+Proof.
+  Admitted.
+(*   intros. *)
+(*   transitivity (<{skip ; p2}>, σ1, φ1). *)
+(*   - now apply seq_star. *)
+(*   - apply clos_rt1n_rtn1. econstructor. *)
+(*     + apply Skip_step. *)
+(*     + apply clos_rtn1_rt1n. *)
+(*       now apply SE_canonical. *)
+(* Qed. *)
+
+Lemma loop_complete: forall p t,
+    (forall (σ : sub) (φ : Bexpr),
+        In _ (denot__S p) (σ, φ) -> (p, id_sub, BTrue) =>* (<{ skip }>, σ, φ)) ->
+    In Trc (traces_of <{ p * }>) t ->
+    (<{ p * }>, id_sub, BTrue) =>* (<{ skip }>, Sub t, PC t).
+Proof.
+  intros p t IH H.
+  destruct H.
+  generalize dependent x.
+  induction i; intros.
+  - inv H; cbn.
+    eexists.
+    split.
+    + econstructor; [ |reflexivity ].
+      apply Loop_step_halt.
+    + auto.
+  - destruct H as (u & v & ? & ? & ->).
+    pose proof IHi _ H0.
+    apply trace_to_denotS in H.
+    apply IH in H.
+    destruct H as (?φ & ? & ?).
+    destruct H1 as (?φ & ? & ?).
+    pose proof seq_canonical _ _ _ _ _ _ H H1 as (?φ & ? & ?).
+    eexists φ1.
+    split.
+    + transitivity (<{ p ; p* }>, id_sub, BTrue).
+      { econstructor; [ |reflexivity ]. constructor. }
+      rewrite sub_trace_app.
+      apply H4.
+    + rewrite pc_trace_app.
+      rewrite H5.
+      rewrite 2 denotB_and.
+      rewrite H2.
+      rewrite 2 inverse_denotB.
+      now rewrite H3.
+Qed.
+
+(* Theorem 5 *)
+Theorem completeness : forall p σ φ,
+    In _ (denot__S p) (σ, φ) ->
+    (p, id_sub, BTrue) =>* (PSkip, σ, φ).
+Proof.
+  induction p; intros;
+    destruct H as (t & DENOT & -> & ->).
+  - inv DENOT.
+    eexists.
+    split; eauto.
+    cbn; constructor.
+  - inv DENOT.
+    eexists.
+    split; auto.
+    cbn.
+    econstructor; [ | reflexivity ].
+    eapply Asgn' with (σ:=id_sub); eauto.
+    now rewrite Aapply_id.
+  - inv DENOT.
+    exists <{BTrue && b}>.
+    split; auto.
+    cbn.
+    econstructor; [ | reflexivity ].
+    eapply Asrt' with (φ:=BTrue) (b:=b); eauto.
+    now rewrite Bapply_id.
+  - destruct DENOT as (u & v & ? & ? & ->).
+    apply trace_to_denotS in H, H0.
+    apply IHp1 in H.
+    destruct H as (?φ & ? & ?).
+    apply IHp2 in H0.
+    destruct H0 as (?φ & ? & ?).
+    assert (In _ (denot__S <{ skip }>) (id_sub, BTrue)) as SKIP by (exists TSkip; split; easy).
+    pose proof canonical_soundness _ _ _ _ _ _ H SKIP as (?φ & ? & ?).
+    pose proof canonical_soundness _ _ _ _ _ _ H0 SKIP as (?φ & ? & ?).
+    pose proof seq_canonical _ _ _ _ _ _ H H0 as (?φ & ? & ?).
+    eexists φ3.
+    split.
+    + rewrite sub_trace_app.
+      apply H7.
+    + rewrite pc_trace_app.
+      rewrite H8.
+      rewrite 2 denotB_and.
+      rewrite H1.
+      rewrite 2 inverse_denotB.
+      now rewrite H2.
+  - inv DENOT.
+    + apply trace_to_denotS in H.
+      apply IHp1 in H.
+      destruct H as (?φ & ? & ?).
+      exists φ.
+      split; auto.
+      etransitivity; [ | apply H ].
+      econstructor; [ |reflexivity ].
+      apply Ndet_step_l.
+    + apply trace_to_denotS in H.
+      apply IHp2 in H.
+      destruct H as (?φ & ? & ?).
+      exists φ.
+      split; auto.
+      etransitivity; [ | apply H ].
+      econstructor; [ |reflexivity ].
+      apply Ndet_step_r.
+  - now apply loop_complete.
+Qed.
+
+Print Assumptions soundness.
+Print Assumptions completeness.
