Programs.v
@@ -1,0 +1,647 @@
+From Coq Require Import
+                 Strings.String
+                 Bool.Bool
+                 Init.Datatypes
+                 Lists.List
+                 Logic.FunctionalExtensionality (* for equality of substitutions *)
+                 Ensembles
+                 Psatz
+                 Classes.RelationClasses.
+
+From BigStepSymbEx Require Import
+  Utils
+  Expr
+  Maps
+  Syntax
+  Traces.
+
+Import NonDet NonDetNotations.
+Import Trace.
+Open Scope com_scope.
+
+(** Concrete semantics *)
+(* Definition 9 *)
+Fixpoint denot_fun_nondet (p: Prg) (V: Valuation): Ensemble Valuation :=
+  match p with
+  | PSkip => Singleton _ V
+  | PAsgn x e => Singleton _ (x !-> Aeval V e ; V)
+  | PAsrt b => if Beval V b then Singleton _ V else Empty_set _ | <{p1 (+) p2}> => Union _ (denot_fun_nondet p1 V) (denot_fun_nondet p2 V)
+  | <{p*}> => Union_Fam (fun n => n_fold_set n (denot_fun_nondet p) V)
+  | PSeq p1 p2 => set_compose (denot_fun_nondet p1) (denot_fun_nondet p2) V
+  end.
+
+(* Lemma 6 *)
+Lemma unfolding_iterations: forall p,
+    denot_fun_nondet <{p*}> = denot_fun_nondet (PChoice PSkip (PSeq p <{p*}>)).
+Proof.
+  intro.
+  extensionality V.
+  apply Extensionality_Ensembles.
+  split;cbn; intros ? ?.
+  - inv H.
+    destruct i.
+    + inv H0.
+      now left.
+    + cbn in H0.
+      right.
+      destruct H0 as (?V & ? & ?).
+      exists V0.
+      split; auto.
+      exists i; auto.
+  - destruct H.
+    + exists 0; auto.
+    + destruct H as (?V & ? & [?n ?V ?]).
+      exists (S n).
+      eexists V0.
+      split; auto.
+Qed.
+
+(*TODO: lemma 7?*)
+
+Definition trace_app (t1 t2: Trc): Trc :=
+  match (t1, t2) with
+  | (TSkip, TSkip) => TSkip
+  | (TSkip, t) => t
+  | (t, TSkip) => t
+  | (t1, t2) => TSeq t1 t2
+  end.
+
+Lemma trace_app_unit_l: forall t, trace_app TSkip t = t.
+Proof. destruct t; auto. Qed.
+
+Lemma trace_app_unit_r: forall t, trace_app t TSkip = t.
+Proof. destruct t; auto. Qed.
+
+Lemma denot_fun_unit_l: forall t, denot_fun t = denot_fun (TSeq TSkip t).
+Proof. destruct t; auto. Qed.
+
+Lemma denot_fun_unit_r: forall t, denot_fun t = denot_fun (TSeq t TSkip).
+Proof.
+  intro.
+  extensionality V.
+  generalize dependent V.
+  induction t; auto.
+  - intros; cbn.
+    now destruct (Beval V b).
+  - simpl; intro.
+    destruct (denot_fun t1 V); simpl; auto.
+    destruct (denot_fun t2 v); simpl; auto.
+Qed.
+
+Lemma trace_app_denot: forall t1 t2,
+    denot_fun (TSeq t1 t2) = denot_fun (trace_app t1 t2).
+Proof.
+  destruct t1, t2; auto.
+  - extensionality V.
+    simpl.
+    destruct (Beval V b); easy.
+  - rewrite trace_app_unit_r.
+    now rewrite <- denot_fun_unit_r.
+Qed.
+
+Lemma trace_app_denot_sub: forall t1 t2,
+    denot_sub (Sub (TSeq t1 t2)) = denot_sub (Sub (trace_app t1 t2)).
+Proof.
+  intros.
+  epose proof Sub_spec_correct (TSeq t1 t2) as (?&_).
+  specialize (H eq_refl).
+  destruct t1, t2; auto; inv H.
+  - inv H3.
+    inv H4.
+    now rewrite compose_subs_id.
+  - inv H3.
+    cbn in *.
+    now rewrite H2, Sub_unit_l.
+  - now rewrite trace_app_unit_r, H2, Sub_unit_r.
+Qed.
+
+Ltac Sub_spec_unfold p :=
+  let H := fresh in epose proof Sub_spec_correct p as (H&_);
+                    specialize (H eq_refl);
+                    inv H.
+
+(* Lemma 2 (ICTAC) *)
+Lemma acc_subst_concat_comp: forall s t,
+    [|(Sub (trace_app s t))|] = fun V => [|(Sub t)|] ([|(Sub s)|] V).
+Proof.
+  destruct s, t; cbn; auto.
+
+  - extensionality V.
+    unfold denot_sub.
+    now rewrite compose_comp.
+
+  - Sub_spec_unfold (TSeq (TAsgn x e) (TSeq t1 t2)).
+    inv H3.
+    extensionality V.
+    unfold denot_sub.
+    rewrite compose_comp.
+    now apply Sub_spec_correct in H4; subst.
+
+  - now rewrite compose_subs_id.
+
+  - Sub_spec_unfold (TSeq (TAsrt b) (TSeq t1 t2)).
+    inv H3.
+    extensionality V.
+    unfold denot_sub.
+    rewrite compose_comp.
+    now apply Sub_spec_correct in H4; subst.
+
+  - Sub_spec_unfold (TSeq (TSeq s1 s2) (TAsgn x e)).
+    inv H4.
+    extensionality V.
+    unfold denot_sub.
+    rewrite compose_comp.
+    now apply Sub_spec_correct in H3; subst.
+
+  - Sub_spec_unfold (TSeq (TSeq s1 s2) (TAsrt b)).
+    inv H4.
+    extensionality V.
+    unfold denot_sub.
+    rewrite compose_comp.
+    now apply Sub_spec_correct in H3; subst.
+
+  - Sub_spec_unfold (TSeq (TSeq s1 s2) (TSeq t1 t2)).
+    rewrite compose_sub_spec.
+    now apply Sub_spec_correct in H3, H4; subst.
+Qed.
+
+Lemma trace_app_denot_pc: forall t1 t2,
+    {| (PC (TSeq t1 t2)) |} = {| (PC (trace_app t1 t2)) |}.
+Proof.
+  intros.
+  epose proof PC_spec_correct (TSeq t1 t2) as (?&_).
+  specialize (H eq_refl).
+  destruct t1, t2; auto; inv H.
+  - inv H3.
+    inv H5.
+    cbn.
+    now rewrite denotB_and, denotB_top, intersect_full, Bapply_id.
+  - inv H3.
+    cbn in *.
+    rewrite denotB_and, denotB_top, intersect_full, Bapply_id.
+    now apply PC_spec_correct in H4; subst.
+  - cbn.
+    now rewrite denotB_and, denotB_top, intersect_comm, intersect_full.
+  - apply PC_spec_correct in H3, H4; subst.
+    cbn.
+    now rewrite denotB_and, denotB_top, intersect_comm, intersect_full.
+Qed.
+
+Ltac PC_spec_unfold p :=
+  let H := fresh in epose proof PC_spec_correct p as (H&_);
+                    specialize (H eq_refl);
+                    inv H.
+
+(* Lemma 3 (ICTAC) *)
+Lemma concat_pc: forall u v,
+    denot__B (PC (trace_app u v)) = denot__B (BAnd (PC u) (Bapply (Sub u) (PC v))).
+Proof.
+  destruct u, v; cbn; auto;
+    try (rewrite denotB_and);
+    try (rewrite denotB_neg);
+    try (rewrite denotB_top);
+    try (rewrite intersect_full);
+    try (rewrite intersect_comm, intersect_full);
+    try (rewrite Bapply_id);
+    auto.
+  - PC_spec_unfold (TSeq (TAsgn x e) (TSeq v1 v2)).
+    apply PC_spec_correct in H3, H4; subst; cbn.
+    now rewrite denotB_and, denotB_top, intersect_full.
+
+  - PC_spec_unfold (TSeq (TAsrt b) (TSeq v1 v2)).
+    apply PC_spec_correct in H3, H4; subst; cbn.
+    now rewrite denotB_and, Bapply_id.
+
+  - PC_spec_unfold (TSeq (TSeq u1 u2) (TAsgn x e)).
+    apply PC_spec_correct in H3, H4; subst; cbn.
+    now rewrite denotB_and, denotB_top, intersect_comm, intersect_full.
+
+  - PC_spec_unfold (TSeq (TSeq u1 u2) (TAsrt b)).
+    apply PC_spec_correct in H3, H4; subst; cbn.
+    now rewrite denotB_and.
+
+  - PC_spec_unfold (TSeq (TSeq u1 u2) (TSeq v1 v2)).
+    rewrite denotB_and.
+    now apply PC_spec_correct in H3, H4; subst.
+Qed.
+
+Fixpoint n_fold_seq (n:nat) (ts: Ensemble Trc): Ensemble Trc :=
+  match n with
+  | 0 => Singleton _ TSkip
+  | S n => fun t => exists u v,
+              In _ ts u
+              /\ In _ (n_fold_seq n ts) v
+              /\  t = trace_app u v
+  end.
+
+(* Definition 10 *)
+Fixpoint traces_of (p:Prg): Ensemble Trc :=
+  match p with
+  | PSkip => Singleton _ TSkip
+  | PAsgn x e => Singleton _ (TAsgn x e)
+  | PAsrt b => Singleton _ (TAsrt b)
+  | <{p1 (+) p2}> => Union _ (traces_of p1) (traces_of p2)
+  | <{p*}> => Union_Fam (fun n => n_fold_seq n (traces_of p))
+  | PSeq p1 p2 => fun x => exists t u, In _ (traces_of p1) t /\ In _ (traces_of p2) u /\ x = trace_app t u
+  end.
+
+Lemma traces_of_loop_step: forall p n u v,
+    In _ (traces_of p) u ->
+    In _ (n_fold_seq n (traces_of p)) v ->
+    In _ (n_fold_seq (S n) (traces_of p)) (trace_app u v).
+Proof.
+  induction n; intros.
+  - cbn in *.
+    inv H0.
+    exists u, TSkip.
+    split; auto.
+  - destruct H0 as (?u & ?v & (? & ? & ->)).
+    pose proof IHn _ _ H H1.
+    exists u, (trace_app u0 v0).
+    split; auto.
+Qed.
+
+(* Lemma 8 *)
+Lemma traces_of_correspondence: forall p V,
+    denot_fun_nondet p V = (fun V' => exists t, denot_fun t V = Some V' /\ In _ (traces_of p) t).
+Proof.
+  intros.
+  apply Extensionality_Ensembles.
+  generalize dependent V.
+  induction p; intros.
+  - split; intros ? ?.
+    + inv H.
+      exists TSkip.
+      split; easy.
+    + destruct H as (t & ? & ?).
+      inv H0.
+      now inv H.
+  - split; intros ? ?.
+    + inv H.
+      exists (TAsgn x e).
+      split; easy.
+    + destruct H as (t & ? & ?).
+      inv H0.
+      now inv H.
+  - split; intros ? ?.
+    + cbn in H.
+      destruct (Beval V b) eqn:?.
+      * inv H.
+        exists (TAsrt b).
+        split; cbn.
+        now rewrite Heqb0.
+        easy.
+      * inv H.
+    + destruct H as (t & ? & ?).
+      inv H0.
+      cbn in *.
+      destruct (Beval V b); [ |discriminate].
+      now inv H.
+  - split; intros ? ?.
+    + destruct H as (?V & ? & ?).
+      apply IHp1 in H.
+      apply IHp2 in H0.
+      destruct H as (?t & ? & ?).
+      destruct H0 as (?t & ? & ?).
+      exists (trace_app t t0).
+      split.
+      * rewrite <- trace_app_denot.
+        cbn.
+        now rewrite H.
+      * exists t, t0.
+        split; auto.
+    + destruct H as (?t & ? & ?).
+      destruct H0 as (u & v & ? & ? & ->).
+      rewrite <- trace_app_denot in H.
+      cbn in *.
+      destruct (option_inversion H) as (?V & ? & ?).
+      assert (exists t, denot_fun t V = Some V0 /\ In _ (traces_of p1) t). {
+        exists u.
+        split; auto.
+      }
+      apply IHp1 in H4.
+      assert (exists t, denot_fun t V0 = Some x /\ In _ (traces_of p2) t). {
+        exists v.
+        split; auto.
+      }
+      apply IHp2 in H5.
+      eexists V0.
+      split; auto.
+  - split; intros ? ?.
+    + destruct H.
+      * apply IHp1 in H.
+        destruct H as (?t & ? & ?).
+        exists t.
+        split; auto.
+        now left.
+      * apply IHp2 in H.
+        destruct H as (?t & ? & ?).
+        exists t.
+        split; auto.
+        now right.
+    + destruct H as (?t & ? & ?).
+      destruct H0.
+      * assert (exists t, denot_fun t V = Some x /\ In _ (traces_of p1) t). {
+          exists x0.
+          split; auto.
+        }
+        apply IHp1 in H1.
+        now left.
+      * assert (exists t, denot_fun t V = Some x /\ In _ (traces_of p2) t). {
+          exists x0.
+          split; auto.
+        }
+        apply IHp2 in H1.
+        now right.
+  - split; intros ? ?.
+    + destruct H as [?n ?V ?].
+      generalize dependent V0.
+      generalize dependent V.
+      induction n; intros.
+      * cbn in H; inv H.
+        exists TSkip.
+        split; auto.
+        exists 0; cbn; easy.
+
+      * destruct H as (?V & ? & ?).
+        destruct (IHp V) as (? & _).
+        destruct (H1 _ H) as (?t & ? & ?).
+
+        destruct (IHn _ _ H0) as (?t & ? & ?).
+        exists (trace_app t t0).
+        split.
+        -- rewrite <- trace_app_denot; simpl.
+           rewrite H2; auto.
+        -- destruct H5 as [?n ? ?].
+           exists (S n0).
+           now apply traces_of_loop_step.
+    + destruct H as (?t & ? & ?).
+      destruct H0 as [?n ? ?].
+      generalize dependent x0.
+      generalize dependent x.
+      generalize dependent V.
+      induction n; intros.
+      * cbn in H0.
+        inv H0.
+        inv H.
+        exists 0; now cbn.
+      * destruct H0 as (?u & ?v & ? & ? & ->).
+        rewrite <- trace_app_denot in H.
+        cbn in H.
+        destruct (option_inversion H) as (?V & ? & ?).
+        pose proof IHn _ _ _ H3 H1.
+        destruct H4 as [?n ? ?].
+
+        pose proof IHp V as (_&?).
+        assert (exists t : Trc, denot_fun t V = Some V0 /\ In Trc (traces_of p) t).
+        {
+          exists u.
+          split; auto.
+        }
+        apply H5 in H6.
+
+        exists (S n0).
+        exists V0.
+        split; auto.
+(* this proof is very ugly, but goes through *)
+Qed.
+
+(** Symbolic Semantics *)
+(* Equation (1) *)
+Lemma denot_sub_sound: forall sigma V e,
+    Aeval (denot_sub sigma V) e = Aeval V (Aapply sigma e).
+Proof. unfold denot_sub. intros. apply comp_sub. Qed.
+
+(* Equation (2) *)
+Lemma inverse_denotB: forall s b,
+    denot__B (Bapply s b) = inverse_image (denot_sub s) (denot__B b).
+Proof.
+  intros. induction b.
+  - simpl. rewrite denotB_top. rewrite inverse_full. reflexivity.
+  - simpl. rewrite denotB_bot. rewrite inverse_empty. reflexivity.
+  - simpl. rewrite 2 denotB_neg. rewrite IHb. rewrite inverse_complement. reflexivity.
+  - simpl. rewrite 2 denotB_and. rewrite IHb1, IHb2. rewrite inverse_intersection. reflexivity.
+  - apply Extensionality_Ensembles. split; intros V H.
+    + inversion H. rewrite <- 2 denot_sub_sound in H1.
+      unfold inverse_image, In. unfold denot_sub. apply H1.
+    + inversion H.
+      unfold denot__B, Ensembles.In. simpl. unfold denot_sub in H1.
+      rewrite <- 2 comp_sub. apply H1.
+Qed.
+
+Definition Branch: Type := sub * Bexpr.
+
+Definition denot__S (p: Prg): Ensemble Branch :=
+  fun '(s, b) => exists t, In _ (traces_of p) t /\ s = Sub t /\ b = PC t.
+
+Lemma sub_trace_app: forall u v,
+    Sub (trace_app u v) = compose_subs (Sub u) (Sub v).
+Proof.
+  destruct u,v; cbn; auto;
+    try (now rewrite compose_subs_id);
+    unfold Sub; cbn.
+    1,2: now destruct (trace_denot__S v1), (trace_denot__S v2); cbn.
+    1,2: now destruct (trace_denot__S u1), (trace_denot__S u2); cbn.
+    now destruct (trace_denot__S u1), (trace_denot__S u2),
+      (trace_denot__S v1), (trace_denot__S v2) ; cbn.
+Qed.
+
+Lemma pc_trace_app: forall u v,
+  {| PC (trace_app u v) |} = {| BAnd (PC u) (Bapply (Sub u) (PC v)) |}.
+  Proof.
+  destruct u,v; cbn; auto;
+    try rewrite Bapply_id;
+    try rewrite denotB_and;
+    try rewrite denotB_top;
+    try rewrite intersect_full;
+    try rewrite intersect_comm, intersect_full;
+    auto.
+  - unfold PC; cbn.
+    destruct (trace_denot__S v1), (trace_denot__S v2); cbn.
+    now rewrite 2 denotB_and, denotB_top, intersect_full.
+  - unfold PC; cbn.
+    destruct (trace_denot__S v1), (trace_denot__S v2); cbn.
+    now rewrite 2 Bapply_id, 2 denotB_and.
+  - unfold PC; cbn.
+    destruct (trace_denot__S u1), (trace_denot__S u2); cbn.
+    now rewrite 2 denotB_and, denotB_top, intersect_comm, intersect_full.
+  - unfold PC; cbn.
+    destruct (trace_denot__S u1) eqn:?, (trace_denot__S u2) eqn:?; cbn.
+    pose proof Sub_spec_correct (TSeq u1 u2) as (?&_).
+    specialize (H eq_refl).
+    inv H.
+    apply Sub_spec_correct in H3, H4.
+    unfold Sub in H3, H4.
+    rewrite Heqp in H3.
+    rewrite Heqp0 in H4.
+    simpl in *; subst.
+    now rewrite denotB_and.
+  - unfold PC; cbn.
+    destruct (trace_denot__S u1) eqn:?, (trace_denot__S u2) eqn:?; cbn.
+    destruct (trace_denot__S v1) eqn:?, (trace_denot__S v2) eqn:?; cbn.
+    pose proof Sub_spec_correct (TSeq u1 u2) as (?&_).
+    specialize (H eq_refl).
+    inv H.
+    apply Sub_spec_correct in H3, H4.
+    unfold Sub in H3, H4.
+    rewrite Heqp in H3.
+    rewrite Heqp0 in H4.
+
+    pose proof Sub_spec_correct (TSeq v1 v2) as (?&_).
+    specialize (H0 eq_refl).
+    inv H0.
+    apply Sub_spec_correct in H7, H8.
+    unfold Sub in H7, H8.
+    rewrite Heqp1 in H7.
+    rewrite Heqp2 in H8.
+    simpl in *; subst.
+    now rewrite 2 denotB_and.
+Qed.
+
+(* Lemma 9 in four parts *)
+Lemma denotS_spec_seq: forall p q,
+    denot__S (PSeq p q) = fun '(σ, φ) => exists σp σq φp φq,
+                            In _ (denot__S p) (σp, φp)
+                            /\ In _ (denot__S q) (σq, φq)
+                            /\ σ = compose_subs σp σq
+                            /\ {|φ|} = {|BAnd φp (Bapply σp φq)|}. (*<- this is an issue *)
+Proof.
+  intros.
+  apply Extensionality_Ensembles.
+  split; intros ? ?.
+  - destruct x.
+    destruct H as (t & ? & -> & ->).
+    destruct H as (u & v & ? & ? & ->).
+    eexists.
+    eexists.
+    eexists.
+    eexists.
+    splits.
+    + eexists.
+      splits; eauto.
+    + eexists.
+      splits; eauto.
+    + apply sub_trace_app.
+    + apply pc_trace_app. (* <- here we only get equal sets *)
+
+  - destruct x.
+    destruct H as (σp & σq & φp & φq & ? & ? & -> & ?).
+    destruct H as (tp & ? & -> & ->).
+    destruct H0 as (tq & ? & -> & ->).
+    eexists (trace_app tp tq).
+    splits.
+    + eexists.
+      eexists.
+      splits; auto.
+    + now rewrite sub_trace_app.
+    + rewrite <- pc_trace_app in H1.
+      admit. (*<- but here the equal sets are not strong enough *)
+Admitted.
+
+Lemma denotS_spec_choice: forall p q,
+    denot__S (PChoice p q) = Union _ (denot__S p) (denot__S q).
+Proof.
+  intros.
+  apply Extensionality_Ensembles.
+  split; intros ? ?.
+  - destruct x.
+    destruct H as (t & ? & -> & ->).
+    destruct H.
+    + left.
+      eexists.
+      splits; auto.
+    + right.
+      eexists.
+      splits; auto.
+  - destruct H.
+    + destruct x.
+      destruct H as (t & ? & -> & ->).
+      eexists.
+      splits; eauto.
+      now left.
+    + destruct x.
+      destruct H as (t & ? & -> & ->).
+      eexists.
+      splits; eauto.
+      now right.
+Qed.
+
+(* TODO: Lemma 9 (iii) *)
+Lemma denotS_spec_unfold: forall p,
+    denot__S (PStar p) = Union _ (denot__S PSkip) (denot__S (PSeq p (PStar p))).
+Proof.
+  intros.
+  apply Extensionality_Ensembles.
+  split; intros ? ?.
+  - destruct x.
+    destruct H as (t & ? & -> & ->).
+    inv H.
+    destruct i.
+    + left.
+      inv H0.
+      eexists.
+      splits; eauto.
+    + destruct H0 as (u & v & ? & ? & ->).
+      right.
+      eexists.
+      splits; eauto.
+      exists u, v.
+      splits; auto.
+      eexists.
+      apply H1.
+  - destruct H.
+    + destruct x.
+      destruct H as (t & ? & -> & ->).
+      inv H.
+      eexists.
+      splits; auto.
+      exists 0; auto.
+    + destruct x.
+      destruct H as (t & ? & -> & ->).
+      destruct H as (u & v & ? & ? & ->).
+      exists (trace_app u v).
+      splits.
+      inv H0.
+      exists (S i).
+      exists u, v.
+      splits; auto.
+Qed.
+
+(* Theorem 3: in two parts *)
+Lemma SE_complete: forall p V V',
+    In _ (denot_fun_nondet p V) V' ->
+    exists s b,
+      In _ (denot__S p) (s, b)
+      /\ (V |= b)
+      /\ ([| s |] V = V').
+Proof.
+  intros.
+  rewrite traces_of_correspondence in H.
+  destruct H as (?t & TRACE_DENOT & IN).
+  apply trace_correspondence in TRACE_DENOT.
+
+  exists (Sub t), (PC t).
+  split; auto.
+  exists t.
+  split; auto.
+Qed.
+
+Lemma SE_correct: forall p V s b,
+    In _ (denot__S p) (s, b) ->
+    V |= b ->
+    In _ (denot_fun_nondet p V) ([| s |] V).
+Proof.
+  intros.
+  cbn in H.
+  destruct H as (?t & ? & -> & ->).
+  rewrite traces_of_correspondence.
+  exists t.
+  split; auto.
+  apply trace_correspondence_aux in H0.
+  now apply trace_sub_correct.
+Qed.
+
+Print Assumptions SE_correct.
+Print Assumptions SE_complete.
+
+(*TODO: Translate results to While *)
