Utils.v
@@ -1,0 +1,264 @@
+From Coq Require Import
+  Ensembles.
+
+From BigStepSymbEx Require Import
+  Maps.
+
+Ltac inv H := inversion H; subst.
+Ltac splits := repeat split.
+
+Section EnsembleHelpers.
+  Context {X Y Z: Type}.
+
+  Definition set_compose (f: X -> Ensemble Y) (g: Y -> Ensemble Z): X -> Ensemble Z :=
+    fun x z => exists y, In _ (f x) y /\ In _ (g y) z.
+
+  Variable A B C: Ensemble X.
+
+  Lemma intersect_full: Intersection X (Full_set _) A = A.
+  Proof.
+    intros. apply Extensionality_Ensembles. split; intros x H.
+    - destruct H; assumption.
+    - split; [constructor | assumption].
+  Qed.
+
+  Lemma intersect_full': Intersection X A (Full_set _) = A.
+  Proof.
+    intros. apply Extensionality_Ensembles. split; intros x H.
+    - destruct H; assumption.
+    - split; [assumption | constructor].
+  Qed.
+
+  Lemma intersect_comm: Intersection _ A B = Intersection _ B A.
+  Proof.
+    intros. apply Extensionality_Ensembles. split; intros x H;
+      destruct H; split; assumption.
+  Qed.
+
+  Lemma intersect_assoc: Intersection _ A (Intersection _ B C) = Intersection _ (Intersection _ A B) C.
+  Proof.
+    intros. apply Extensionality_Ensembles. split; intros x H; repeat split;
+      try (destruct H; destruct H0; assumption);
+      destruct H; destruct H; assumption.
+  Qed.
+
+  Definition inverse_image {X: Type} (F: X -> X) (B: Ensemble X): Ensemble X := fun x => B (F x).
+
+  (* characterizing inverse images *)
+  Lemma inverse_id : forall (A: Ensemble X), inverse_image (fun x => x)  A = A.
+  Proof. intros. apply Extensionality_Ensembles. split; intros V H; assumption. Qed.
+
+  Lemma inverse_full : forall F, inverse_image F (Full_set _) = Full_set X.
+  Proof. intros. apply Extensionality_Ensembles. split; intros V _; constructor. Qed.
+
+  Lemma inverse_empty : forall F, inverse_image F (Empty_set _) = Empty_set X.
+  Proof. intros. apply Extensionality_Ensembles. split; intros V H; inversion H. Qed.
+
+  Lemma inverse_complement : forall F B,
+      inverse_image F (Complement _ B) = Complement X (inverse_image F B).
+  Proof.
+    intros. apply Extensionality_Ensembles. split; intros V H.
+    - intro contra. apply H. apply contra.
+    - apply H.
+  Qed.
+
+  Lemma inverse_intersection : forall F B1 B2,
+      inverse_image F (Intersection _ B1 B2) = Intersection X (inverse_image F B1) (inverse_image F B2).
+  Proof.
+    intros. apply Extensionality_Ensembles. split; intros V H.
+    - inversion H; subst. split; assumption.
+    - destruct H. split; assumption.
+  Qed.
+
+  Lemma inverse_inverse : forall F F' (B: Ensemble X),
+      inverse_image F (inverse_image F' B) = inverse_image (fun x => F' (F x)) B.
+  Proof.
+    intros. apply Extensionality_Ensembles. split; intros V H.
+    - apply H.
+    - apply H.
+  Qed.
+
+  Inductive Union_Fam {X I} (Fs: I -> Ensemble X): Ensemble X :=
+    | Fam_intro: forall {i x}, In _ (Fs i) x -> In _ (Union_Fam Fs) x.
+
+Lemma set_compose_singleton (f: X -> Ensemble Y) (g: Y -> Ensemble Z):
+  forall x y z, f x = Singleton _ y -> g y = Singleton _ z ->
+           set_compose f g x = Singleton _ z.
+Proof.
+  intros.
+  apply Extensionality_Ensembles.
+  split; intros ? ?.
+  - inv H1.
+    destruct H2.
+    rewrite H in H2.
+    inv H2.
+    rewrite H0 in H3.
+    inv H3.
+    easy.
+  - inv H1.
+    unfold set_compose.
+    unfold In.
+    exists y.
+    split.
+    + now rewrite H.
+    + now rewrite H0.
+Qed.
+
+Lemma singleton_inv: forall x x', Singleton X x = Singleton X x' <-> x = x'.
+Proof.
+  split; intro.
+  - assert (Same_set _ (Singleton _ x) (Singleton _ x')). {
+      split; intros ? ?.
+      + inv H0.
+        now rewrite <- H.
+      + now rewrite H, H0.
+    }
+    inv H0.
+    assert (In _ (Singleton _ x') x). {
+      now apply (H1 x).
+    }
+    now inv H3.
+  - now rewrite H.
+Qed.
+
+End EnsembleHelpers.
+
+#[export] Hint Rewrite (@intersect_comm Valuation) (@intersect_full Valuation) : denotB.
+
+From Coq Require Import
+  Relations
+  Classes.RelationClasses
+  Relations.Operators_Properties.
+Section RelationHelpers.
+  Variable A: Type.
+  Variable R: relation A.
+
+  Lemma clos_rtn1_rt1n: forall x y,
+      clos_refl_trans_n1 _ R x y -> clos_refl_trans_1n _ R x y.
+  Proof. intros. apply clos_rt_rt1n. apply clos_rtn1_rt. apply H. Qed.
+
+  Lemma clos_rt1n_rtn1: forall x y,
+      clos_refl_trans_1n _ R x y -> clos_refl_trans_n1 _ R x y.
+  Proof. intros. apply clos_rt_rtn1. apply clos_rt1n_rt. apply H. Qed.
+
+  Lemma clos_rt1n_rtn1_iff: forall x y,
+      clos_refl_trans_1n _ R x y <-> clos_refl_trans_n1 _ R x y.
+  Proof. split; [apply clos_rt1n_rtn1 | apply clos_rtn1_rt1n]. Qed.
+
+  Global Instance clos_rtn1_trans: Transitive (clos_refl_trans_n1 _ R).
+  Proof.
+    intros x y z H0 H1.
+    apply clos_rtn1_rt in H0, H1.
+    apply clos_rt_rtn1.
+    apply rt_trans with (y := y); assumption.
+  Qed.
+
+  Global Instance clos_rtn1_refl: Reflexive (clos_refl_trans_n1 _ R).
+  Proof.
+    intro. constructor.
+  Qed.
+End RelationHelpers.
+
+From Coq Require Import
+  Init.Datatypes
+  Lists.List.
+
+Section ListHelpers.
+  Import ListNotations.
+  Open Scope list_scope.
+  Variable A : Type.
+
+  Lemma app_tail_inj: forall (t1 t2 t2': list A),
+      t1 ++ t2 = t1 ++ t2' -> t2 = t2'.
+  Proof.
+    induction t1; intros.
+    - apply H.
+    - simpl in H. inversion H.
+      apply IHt1; assumption.
+  Qed.
+
+  Lemma app_nil_unique_r: forall (t1 t2: list A),
+      t1 = t1 ++ t2 -> t2 = [].
+  Proof.
+    induction t1; intros.
+    - rewrite H. auto.
+    - inversion H. apply IHt1; assumption.
+  Qed.
+
+  Lemma app_nil_unique_l: forall (t1 t2: list A),
+      t1 = t2 ++ t1 -> t2 = [].
+  Proof.
+    induction t1; intros.
+    - rewrite app_nil_r in H. auto.
+    - destruct t2; auto.
+      inversion H; subst. replace (t2 ++ a0 :: t1) with ((t2 ++ [a0]) ++ t1) in H2.
+      + apply IHt1 in H2. destruct (app_eq_nil _ _ H2); subst; assumption.
+      + rewrite <- app_assoc. auto.
+  Qed.
+End ListHelpers.
+
+Definition option_bind {X Y: Type} (m : option X) (f: X -> option Y): option Y :=
+  match m with None => None | Some x => f x end.
+
+Definition option_compose {X Y Z: Type} (f: X -> option Y) (g: Y -> option Z): X -> option Z :=
+  fun x => option_bind (f x) g.
+
+Definition option_lift {X Y: Type} (f: X -> Y): X -> option Y := fun x => Some (f x).
+
+(* Lemma option_bind_mono: forall (X Y: Type) (x x': option X) (f f': X -> option Y), *)
+(*     x <<= x' -> (forall x, f x <<= f' x) -> option_bind x f <<= option_bind x' f'. *)
+(* Proof. intros. destruct H; cbn; auto with lessdef. Qed. *)
+
+Lemma option_inversion {X Y: Type} {x: option X} {f: X -> option Y} {y: Y}:
+  option_bind x f = Some y ->
+  exists x', x = Some x' /\ f x' = Some y.
+Proof.
+  destruct x; simpl; intros.
+  - exists x. split; auto.
+  - inversion H.
+Qed.
+Lemma some_not_none {X:Type}: forall (x:X), Some x <> None.
+Proof. easy. Qed.
+
+Lemma option_inversion_none {X Y: Type}: forall (x: option X) (f: X -> option Y),
+    option_bind x f = None ->
+    x = None \/ exists y, x = Some y /\ f y = None.
+Proof.
+  intros.
+  destruct x.
+  - cbn in H.
+    right.
+    exists x.
+    split; auto.
+  - now left.
+Qed.
+
+Fixpoint n_fold {X: Type} (n: nat) (f: X -> X): X -> X :=
+  match n with
+  | 0 => fun x => x
+  | S n => fun x => f (n_fold n f x)
+  end.
+
+Lemma n_fold_inversion {X:Type}: forall n f (x: X), f (n_fold n f x) = n_fold (S n) f x.
+Proof. reflexivity. Qed.
+
+Lemma n_fold_step {X:Type}: forall n f (x y: X), n_fold (S n) f x = y -> exists z, n_fold n f x = z /\ f z = y.
+Proof.
+    induction n; intros; simpl in *.
+    - exists x. split; [reflexivity | apply H].
+    - exists (f (n_fold n f x)). split; [reflexivity | apply H].
+Qed.
+
+Lemma n_fold_construct {X:Type}: forall n f (x y z: X),
+    n_fold n f x = y -> f y = z -> n_fold (S n) f x = z.
+Proof.
+    induction n; intros; simpl in *.
+    - rewrite H. apply H0.
+    - rewrite (IHn f x (n_fold n f x) y); auto.
+Qed.
+
+Fixpoint n_fold_set {X: Type} (n: nat) (f: X -> Ensemble X): X -> Ensemble X :=
+  match n with
+  | 0 => Singleton _
+  | S n => set_compose f (n_fold_set n f)
+  end.
